Strata/DDM/Integration/Lean/ToExpr.lean
@@ -19,6 +19,18 @@ namespace Strata
 
 open Lean
 
+namespace SepFormat
+
+instance : ToExpr SepFormat where
+  toTypeExpr := private mkConst ``SepFormat
+  toExpr
+    | .none => mkConst ``SepFormat.none
+    | .comma => mkConst ``SepFormat.comma
+    | .space => mkConst ``SepFormat.space
+    | .spacePrefix => mkConst ``SepFormat.spacePrefix
+
+end SepFormat
+
 namespace QualifiedIdent
 
 instance : ToExpr QualifiedIdent where
@@ -159,12 +171,9 @@ private def ArgF.toExpr {α} [ToExpr α] : ArgF α → Lean.Expr
 | .option ann a =>
   let tpe := ArgF.typeExpr α
   astAnnExpr! ArgF.option ann (optionToExpr tpe <| a.attach.map fun ⟨e, _⟩ => e.toExpr)
-| .seq ann a =>
+| .seq ann sep a =>
   let tpe := ArgF.typeExpr α
-  astAnnExpr! ArgF.seq ann <| arrayToExpr .zero tpe <| a.map (·.toExpr)
-| .commaSepList ann a =>
-  let tpe := ArgF.typeExpr α
-  astAnnExpr! ArgF.commaSepList ann <| arrayToExpr .zero tpe <| a.map (·.toExpr)
+  astAnnExpr! ArgF.seq ann (toExpr sep) <| arrayToExpr .zero tpe <| a.map (·.toExpr)
 termination_by a => sizeOf a
 
 private protected def OperationF.toExpr {α} [ToExpr α] (op : OperationF α) : Lean.Expr :=
