Strata/Languages/Boogie/DDMTransform/Translate.lean
@@ -89,7 +89,7 @@ def checkOpArg (arg : Arg) (name : QualifiedIdent) (argc : Nat) : TransM (Array 
 
 def translateCommaSep [Inhabited α] (f : Strata.Arg → TransM α) (arg : Strata.Arg) :
   TransM (Array α) := do
-  let .commaSepList _ args := arg
+  let .seq _ .comma args := arg
     | TransM.error s!"Expected commaSepList: {repr arg}"
   args.mapM f
 
@@ -300,7 +300,7 @@ def translateTypeSynonym (bindings : TransBindings) (op : Operation) :
               let bargs ← checkOpArg arg q`Boogie.mkBindings 1
               let args ←
                   match bargs[0]! with
-                  | .commaSepList _ args =>
+                  | .seq _ .comma args =>
                     let (arr, bindings) ← translateTypeBindings bindings args
                     return (arr.toList, bindings)
                   | _ => TransM.error
@@ -325,7 +325,7 @@ def translateTypeDecl (bindings : TransBindings) (op : Operation) :
               let bargs ← checkOpArg arg q`Boogie.mkBindings 1
               let numargs ←
                   match bargs[0]! with
-                  | .commaSepList _ args => pure args.size
+                  | .seq _ .comma args => pure args.size
                   | _ => TransM.error
                           s!"translateTypeDecl expects a comma separated list: {repr bargs[0]!}")
                     op.args[1]!
@@ -1024,7 +1024,7 @@ partial def translateStmt (p : Program) (bindings : TransBindings) (arg : Arg) :
 partial def translateBlock (p : Program) (bindings : TransBindings) (arg : Arg) :
   TransM ((List Boogie.Statement) × TransBindings) := do
   let args ← checkOpArg arg q`Boogie.block 1
-  let .seq _ stmts := args[0]!
+  let .seq _ .none stmts := args[0]!
     | TransM.error s!"Invalid block {repr args[0]!}"
   let (a, bindings) ← stmts.foldlM (init := (#[], bindings)) fun (a, b) s => do
       let (s, b) ← translateStmt p b s
@@ -1064,7 +1064,7 @@ def translateBindings (bindings : TransBindings) (op : Arg) :
   TransM (ListMap BoogieIdent LMonoTy) := do
   let bargs ← checkOpArg op q`Boogie.mkBindings 1
   match bargs[0]! with
-  | .commaSepList _ args =>
+  | .seq _ .comma args =>
     let arr ← translateInitMkBindings bindings args
     return arr.toList
   | _ =>
@@ -1121,7 +1121,7 @@ def translateSpecElem (p : Program) (name : BoogieIdent) (count : Nat) (bindings
 partial def translateSpec (p : Program) (name : BoogieIdent) (bindings : TransBindings) (arg : Arg) :
   TransM (List BoogieIdent × ListMap BoogieLabel Procedure.Check × ListMap BoogieLabel Procedure.Check) := do
   let sargs ← checkOpArg arg q`Boogie.spec_mk 1
-  let .seq _ args := sargs[0]!
+  let .seq _ .none args := sargs[0]!
     | TransM.error s!"Invalid specs {repr sargs[0]!}"
   go 0 args.size args
   where go (count max : Nat) (args : Array Arg) := do
@@ -1332,7 +1332,7 @@ def translateDatatype (p : Program) (bindings : TransBindings) (op : Operation) 
               let bargs ← checkOpArg arg q`Boogie.mkBindings 1
               let args ←
                   match bargs[0]! with
-                  | .commaSepList _ args =>
+                  | .seq _ .comma args =>
                     let (arr, bindings) ← translateTypeBindings bindings args
                     return (arr.toList, bindings)
                   | _ => TransM.error
